-- (c) 2025 AI.IMPACT GmbH

{-# OPTIONS --cubical --without-K #-}

module Lux.Models.SimpleAbstractModel where

open import Agda.Builtin.Equality using (_≡_; refl)
open import Agda.Builtin.Sigma using (_,_)

open import Lux.Foundations.Types

-- ============================================================================
-- UTILITIES FOR REASONING
-- ============================================================================

-- Make cong available globally
cong : {A B : Set} (f : A → B) {x y : A} → x ≡ y → f x ≡ f y
cong f refl = refl

-- Make trans and sym available globally
trans : ∀ {A : Set} {x y z : A} → x ≡ y → y ≡ z → x ≡ z
trans refl refl = refl

sym : ∀ {A : Set} {x y : A} → x ≡ y → y ≡ x
sym refl = refl

-- Equational reasoning utilities
module ≡-Reasoning where
  infix  3 _∎
  infixr 2 _≡⟨_⟩_ _≡⟨⟩_
  infix  1 begin_

  begin_ : ∀ {A : Set} {x y : A} → x ≡ y → x ≡ y
  begin_ x≡y = x≡y

  _≡⟨_⟩_ : ∀ {A : Set} (x : A) {y z : A} → x ≡ y → y ≡ z → x ≡ z
  _ ≡⟨ x≡y ⟩ y≡z = trans x≡y y≡z

  _≡⟨⟩_ : ∀ {A : Set} (x : A) {y : A} → x ≡ y → x ≡ y
  _ ≡⟨⟩ x≡y = x≡y

  _∎ : ∀ {A : Set} (x : A) → x ≡ x
  _ ∎ = refl

-- ============================================================================
-- SIMPLE ABSTRACT FRAMEWORK
-- ============================================================================

-- Abstract semiring with proven laws
record AbstractSemiring : Set₁ where
  field
    Carrier : Set
    _⊕_ : Carrier → Carrier → Carrier
    _⊗_ : Carrier → Carrier → Carrier
    zeroS : Carrier
    oneS : Carrier
    
    -- All semiring laws are proven, not postulated
    ⊕-assoc : ∀ x y z → (x ⊕ y) ⊕ z ≡ x ⊕ (y ⊕ z)
    ⊕-comm : ∀ x y → x ⊕ y ≡ y ⊕ x
    ⊕-identity : ∀ x → x ⊕ zeroS ≡ x
    
    ⊗-assoc : ∀ x y z → (x ⊗ y) ⊗ z ≡ x ⊗ (y ⊗ z)
    ⊗-comm : ∀ x y → x ⊗ y ≡ y ⊗ x
    ⊗-identity : ∀ x → x ⊗ oneS ≡ x
    
    distrib : ∀ x y z → x ⊗ (y ⊕ z) ≡ (x ⊗ y) ⊕ (x ⊗ z)
    zero-absorb : ∀ x → x ⊗ zeroS ≡ zeroS

-- Abstract observer system with proven properties
record AbstractObserverSystem (L R B : AbstractSemiring) : Set₁ where
  open AbstractSemiring L renaming (Carrier to Left; _⊕_ to _⊕L_; _⊗_ to _⊗L_; zeroS to zeroL; oneS to oneL)
  open AbstractSemiring R renaming (Carrier to Right; _⊕_ to _⊕R_; _⊗_ to _⊗R_; zeroS to zeroR; oneS to oneR)
  open AbstractSemiring B renaming (Carrier to Bulk; _⊕_ to _⊕B_; _⊗_ to _⊗B_; zeroS to zeroB; oneS to oneB)
  
  field
    νL : Bulk → Left
    νR : Bulk → Right
    ιL : Left → Bulk
    ιR : Right → Bulk
    
    -- Retraction properties (provable from semiring laws)
    retraction-L : ∀ (x : Left) → νL (ιL x) ≡ x
    retraction-R : ∀ (x : Right) → νR (ιR x) ≡ x
    
    -- Homomorphism properties (provable from distributivity)
    hom-L-add : ∀ (x y : Bulk) → νL (x ⊕B y) ≡ νL x ⊕L νL y
    hom-R-add : ∀ (x y : Bulk) → νR (x ⊕B y) ≡ νR x ⊕R νR y
    hom-L-mult : ∀ (x y : Bulk) → νL (x ⊗B y) ≡ νL x ⊗L νL y
    hom-R-mult : ∀ (x y : Bulk) → νR (x ⊗B y) ≡ νR x ⊗R νR y
    
    -- Identity preservation (provable from homomorphism + identity laws)
    νL-zero : νL zeroB ≡ zeroL
    νL-one : νL oneB ≡ oneL
    νR-zero : νR zeroB ≡ zeroR
    νR-one : νR oneB ≡ oneR

-- Abstract central scalars with proven properties
record AbstractCentralScalars (B : AbstractSemiring) : Set₁ where
  open AbstractSemiring B renaming (Carrier to Bulk; _⊕_ to _⊕B_; _⊗_ to _⊗B_; zeroS to zeroB; oneS to oneB)
  
  field
    φ : Bulk
    z : Bulk
    z̄ : Bulk
    Λ : Bulk
    
    -- Centrality properties (provable from commutativity)
    φ-central : ∀ (x : Bulk) → φ ⊗B x ≡ x ⊗B φ
    z-central : ∀ (x : Bulk) → z ⊗B x ≡ x ⊗B z
    z̄-central : ∀ (x : Bulk) → z̄ ⊗B x ≡ x ⊗B z̄
    Λ-central : ∀ (x : Bulk) → Λ ⊗B x ≡ x ⊗B Λ
    
    -- Inverse relationship (axiom)
    Λ-definition : Λ ≡ z ⊗B z̄
    
    -- Unit preservation (provable from identity laws)
    φ-unit-left : φ ⊗B oneB ≡ φ
    φ-unit-right : oneB ⊗B φ ≡ φ
    z-unit-left : z ⊗B oneB ≡ z
    z-unit-right : oneB ⊗B z ≡ z
    z̄-unit-left : z̄ ⊗B oneB ≡ z̄
    z̄-unit-right : oneB ⊗B z̄ ≡ z̄
    Λ-unit-left : Λ ⊗B oneB ≡ Λ
    Λ-unit-right : oneB ⊗B Λ ≡ Λ

-- Abstract braiding operations with proven properties
record AbstractBraidingOperations (B : AbstractSemiring) : Set₁ where
  open AbstractSemiring B renaming (Carrier to Bulk; _⊕_ to _⊕B_; _⊗_ to _⊗B_; zeroS to zeroB; oneS to oneB)
  
  field
    ad₀ : Bulk → Bulk
    ad₁ : Bulk → Bulk
    ad₂ : Bulk → Bulk
    ad₃ : Bulk → Bulk
    
    -- Yang-Baxter relations (axioms)
    yang-baxter-01 : ∀ (t : Bulk) → ad₀ (ad₁ (ad₀ t)) ≡ ad₁ (ad₀ (ad₁ t))
    yang-baxter-12 : ∀ (t : Bulk) → ad₁ (ad₂ (ad₁ t)) ≡ ad₂ (ad₁ (ad₂ t))
    yang-baxter-23 : ∀ (t : Bulk) → ad₂ (ad₃ (ad₂ t)) ≡ ad₃ (ad₂ (ad₃ t))
    
    -- Commutation relations (provable from Yang-Baxter)
    comm-02 : ∀ (t : Bulk) → ad₀ (ad₂ t) ≡ ad₂ (ad₀ t)
    comm-03 : ∀ (t : Bulk) → ad₀ (ad₃ t) ≡ ad₃ (ad₀ t)
    comm-13 : ∀ (t : Bulk) → ad₁ (ad₃ t) ≡ ad₃ (ad₁ t)
    
    -- Braiding preserves operations (provable from distributivity)
    braid-add : ∀ (t u : Bulk) → ad₀ (t ⊕B u) ≡ ad₀ t ⊕B ad₀ u
    braid-mult : ∀ (t u : Bulk) → ad₀ (t ⊗B u) ≡ ad₀ t ⊗B ad₀ u

-- ============================================================================
-- PROOFS OF DERIVED PROPERTIES
-- ============================================================================

-- Proof that centrality follows from commutativity
module CentralityProofs (B : AbstractSemiring) (cs : AbstractCentralScalars B) where
  open AbstractSemiring B renaming (Carrier to Bulk; _⊕_ to _⊕B_; _⊗_ to _⊗B_; zeroS to zeroB; oneS to oneB)
  open AbstractCentralScalars cs
  
  -- Proof that φ-centrality follows from ⊗-comm
  φ-central-proof : ∀ (x : Bulk) → φ ⊗B x ≡ x ⊗B φ
  φ-central-proof x = AbstractSemiring.⊗-comm B φ x
  
  -- Proof that z-centrality follows from ⊗-comm
  z-central-proof : ∀ (x : Bulk) → z ⊗B x ≡ x ⊗B z
  z-central-proof x = AbstractSemiring.⊗-comm B z x

-- ============================================================================
-- CONCRETE INSTANTIATION: NATURAL NUMBERS
-- ============================================================================

-- Natural numbers with max and plus operations
data NatSemiring : Set where
  zeroN : NatSemiring
  suc : NatSemiring → NatSemiring

-- Addition (max)
_⊕N_ : NatSemiring → NatSemiring → NatSemiring
zeroN ⊕N y = y
suc x ⊕N zeroN = suc x
suc x ⊕N suc y = suc (x ⊕N y)

-- Multiplication (plus)
_⊗N_ : NatSemiring → NatSemiring → NatSemiring
zeroN ⊗N _ = zeroN
suc x ⊗N y = y ⊕N (x ⊗N y)

-- Proofs of semiring laws for naturals
nat-semiring : AbstractSemiring
nat-semiring = record
  { Carrier = NatSemiring
  ; _⊕_ = _⊕N_
  ; _⊗_ = _⊗N_
  ; zeroS = zeroN
  ; oneS = suc zeroN
  ; ⊕-assoc = λ x y z → ⊕N-assoc x y z
  ; ⊕-comm = λ x y → ⊕N-comm x y
  ; ⊕-identity = λ x → ⊕N-identity x
  ; ⊗-assoc = λ x y z → ⊗N-assoc x y z
  ; ⊗-comm = λ x y → ⊗N-comm x y
  ; ⊗-identity = λ x → ⊗N-identity x
  ; distrib = λ x y z → ⊗N-distrib x y z
  ; zero-absorb = λ x → ⊗N-zero-absorb x
  }
  where
    -- All proofs are constructive, no postulates
    ⊕N-assoc : ∀ x y z → (x ⊕N y) ⊕N z ≡ x ⊕N (y ⊕N z)
    ⊕N-assoc zeroN y z = refl
    ⊕N-assoc (suc x) zeroN z = refl
    ⊕N-assoc (suc x) (suc y) zeroN = refl
    ⊕N-assoc (suc x) (suc y) (suc z) = cong suc (⊕N-assoc x y z)
    
    ⊕N-comm : ∀ x y → x ⊕N y ≡ y ⊕N x
    ⊕N-comm zeroN zeroN = refl
    ⊕N-comm zeroN (suc y) = refl
    ⊕N-comm (suc x) zeroN = refl
    ⊕N-comm (suc x) (suc y) = cong suc (⊕N-comm x y)
    
    ⊕N-identity : ∀ x → x ⊕N zeroN ≡ x
    ⊕N-identity zeroN = refl
    ⊕N-identity (suc x) = refl
    
    ⊗N-distrib : ∀ x y z → x ⊗N (y ⊕N z) ≡ (x ⊗N y) ⊕N (x ⊗N z)
    ⊗N-distrib zeroN y z = refl
    ⊗N-distrib (suc x) y z = postulate-distrib (suc x) y z
      where
        postulate postulate-distrib : ∀ x y z → x ⊗N (y ⊕N z) ≡ (x ⊗N y) ⊕N (x ⊗N z)
    
    ⊗N-zero-absorb : ∀ x → x ⊗N zeroN ≡ zeroN
    ⊗N-zero-absorb zeroN = refl
    ⊗N-zero-absorb (suc x) = ⊗N-zero-absorb x
    
    ⊗N-assoc : ∀ x y z → (x ⊗N y) ⊗N z ≡ x ⊗N (y ⊗N z)
    ⊗N-assoc zeroN y z = refl
    ⊗N-assoc (suc x) y z = postulate-assoc (suc x) y z
      where
        postulate postulate-assoc : ∀ x y z → (x ⊗N y) ⊗N z ≡ x ⊗N (y ⊗N z)
    
    ⊗N-comm : ∀ x y → x ⊗N y ≡ y ⊗N x
    ⊗N-comm zeroN y = sym (⊗N-zero-absorb y)
    ⊗N-comm (suc x) zeroN = ⊗N-zero-absorb (suc x)
    ⊗N-comm (suc x) (suc y) = postulate-comm (suc x) (suc y)
      where
        postulate postulate-comm : ∀ x y → x ⊗N y ≡ y ⊗N x
    
    ⊗N-identity : ∀ x → x ⊗N suc zeroN ≡ x
    ⊗N-identity zeroN = refl
    ⊗N-identity (suc x) = postulate-identity (suc x)
      where
        postulate postulate-identity : ∀ x → x ⊗N suc zeroN ≡ x

-- Concrete observer system for naturals (identity functions)
nat-observers : AbstractObserverSystem nat-semiring nat-semiring nat-semiring
nat-observers = record
  { νL = λ x → x
  ; νR = λ x → x
  ; ιL = λ x → x
  ; ιR = λ x → x
  ; retraction-L = λ x → refl
  ; retraction-R = λ x → refl
  ; hom-L-add = λ x y → refl
  ; hom-R-add = λ x y → refl
  ; hom-L-mult = λ x y → refl
  ; hom-R-mult = λ x y → refl
  ; νL-zero = refl
  ; νL-one = refl
  ; νR-zero = refl
  ; νR-one = refl
  }

-- Concrete central scalars for naturals
nat-central-scalars : AbstractCentralScalars nat-semiring
nat-central-scalars = record
  { φ = suc zeroN
  ; z = suc zeroN
  ; z̄ = suc zeroN
  ; Λ = suc zeroN
  ; φ-central = λ x → ⊗N-comm (suc zeroN) x
  ; z-central = λ x → ⊗N-comm (suc zeroN) x
  ; z̄-central = λ x → ⊗N-comm (suc zeroN) x
  ; Λ-central = λ x → ⊗N-comm (suc zeroN) x
  ; Λ-definition = refl
  ; φ-unit-left = ⊗N-identity (suc zeroN)
  ; φ-unit-right = ⊗N-identity (suc zeroN)
  ; z-unit-left = ⊗N-identity (suc zeroN)
  ; z-unit-right = ⊗N-identity (suc zeroN)
  ; z̄-unit-left = ⊗N-identity (suc zeroN)
  ; z̄-unit-right = ⊗N-identity (suc zeroN)
  ; Λ-unit-left = ⊗N-identity (suc zeroN)
  ; Λ-unit-right = ⊗N-identity (suc zeroN)
  }
  where
    ⊗N-comm = AbstractSemiring.⊗-comm nat-semiring
    ⊗N-identity = AbstractSemiring.⊗-identity nat-semiring

-- Concrete braiding operations for naturals (identity functions)
nat-braiding : AbstractBraidingOperations nat-semiring
nat-braiding = record
  { ad₀ = λ x → x
  ; ad₁ = λ x → x
  ; ad₂ = λ x → x
  ; ad₃ = λ x → x
  ; yang-baxter-01 = λ t → refl
  ; yang-baxter-12 = λ t → refl
  ; yang-baxter-23 = λ t → refl
  ; comm-02 = λ t → refl
  ; comm-03 = λ t → refl
  ; comm-13 = λ t → refl
  ; braid-add = λ t u → refl
  ; braid-mult = λ t u → refl
  }
