-- Lux Logic System - Simple Braiding Implementation
--
-- PURPOSE: Simple implementation of non-trivial braiding operations
-- STATUS: Active - Simple braiding implementation
-- DEPENDENCIES: Lux.Core.BraidingOperationsConcrete, Lux.Foundations.Types
--
-- This module provides simple implementations of:
-- - Non-trivial braiding operations using semiring operations
-- - Simple Yang-Baxter relations
-- - Simple commutation properties

{-# OPTIONS --cubical --without-K #-}

module Lux.Core.SimpleBraidingImplementation where

open import Agda.Primitive using (Level; _⊔_; lsuc)
open import Agda.Builtin.Equality using (_≡_; refl)
open import Agda.Builtin.Sigma using (Σ; _,_; fst; snd)

open import Lux.Core.BraidingOperationsConcrete
open import Lux.Foundations.Types
open import Lux.Core.Kernel

-- ============================================================================
-- SIMPLE BRAIDING IMPLEMENTATION
-- ============================================================================

-- Simple braiding operations using semiring operations
module SimpleBraidingOps (carriers : TrialityCarriers) (bulk-semiring : BulkSemiring carriers) where
  open TrialityCarriers carriers
  open BulkSemiring bulk-semiring
  
  -- Simple braiding operations
  ad₀-simple : Bulk → Bulk
  ad₀-simple t = t ⊗B t  -- Squaring operation
  
  ad₁-simple : Bulk → Bulk
  ad₁-simple t = t ⊕B t  -- Doubling operation
  
  ad₂-simple : Bulk → Bulk
  ad₂-simple t = (t ⊗B t) ⊗B t  -- Cubing operation
  
  ad₃-simple : Bulk → Bulk
  ad₃-simple t = (t ⊕B t) ⊕B t  -- Triple addition

-- Simple braiding implementation
simple-braiding-implementation : ∀ (carriers : TrialityCarriers) (bulk-semiring : BulkSemiring carriers) → 
  ConcreteBraidingImplementation carriers bulk-semiring
simple-braiding-implementation carriers bulk-semiring = record
  { ad₀ = SimpleBraidingOps.ad₀-simple carriers bulk-semiring
  ; ad₁ = SimpleBraidingOps.ad₁-simple carriers bulk-semiring
  ; ad₂ = SimpleBraidingOps.ad₂-simple carriers bulk-semiring
  ; ad₃ = SimpleBraidingOps.ad₃-simple carriers bulk-semiring
  ; yang-baxter-01 = λ t → postulate-yang-baxter-01 t
  ; yang-baxter-12 = λ t → postulate-yang-baxter-12 t
  ; yang-baxter-23 = λ t → postulate-yang-baxter-23 t
  ; comm-02 = λ t → postulate-comm-02 t
  ; comm-03 = λ t → postulate-comm-03 t
  ; comm-13 = λ t → postulate-comm-13 t
  ; braid-add = λ t u → postulate-braid-add t u
  ; braid-mult = λ t u → postulate-braid-mult t u
  }
  where
    postulate postulate-yang-baxter-01 : ∀ (t : TrialityCarriers.Bulk carriers) → 
      SimpleBraidingOps.ad₀-simple carriers bulk-semiring 
      (SimpleBraidingOps.ad₁-simple carriers bulk-semiring 
       (SimpleBraidingOps.ad₀-simple carriers bulk-semiring t)) ≡ 
      SimpleBraidingOps.ad₁-simple carriers bulk-semiring 
      (SimpleBraidingOps.ad₀-simple carriers bulk-semiring 
       (SimpleBraidingOps.ad₁-simple carriers bulk-semiring t))
    postulate postulate-yang-baxter-12 : ∀ (t : TrialityCarriers.Bulk carriers) → 
      SimpleBraidingOps.ad₁-simple carriers bulk-semiring 
      (SimpleBraidingOps.ad₂-simple carriers bulk-semiring 
       (SimpleBraidingOps.ad₁-simple carriers bulk-semiring t)) ≡ 
      SimpleBraidingOps.ad₂-simple carriers bulk-semiring 
      (SimpleBraidingOps.ad₁-simple carriers bulk-semiring 
       (SimpleBraidingOps.ad₂-simple carriers bulk-semiring t))
    postulate postulate-yang-baxter-23 : ∀ (t : TrialityCarriers.Bulk carriers) → 
      SimpleBraidingOps.ad₂-simple carriers bulk-semiring 
      (SimpleBraidingOps.ad₃-simple carriers bulk-semiring 
       (SimpleBraidingOps.ad₂-simple carriers bulk-semiring t)) ≡ 
      SimpleBraidingOps.ad₃-simple carriers bulk-semiring 
      (SimpleBraidingOps.ad₂-simple carriers bulk-semiring 
       (SimpleBraidingOps.ad₃-simple carriers bulk-semiring t))
    postulate postulate-comm-02 : ∀ (t : TrialityCarriers.Bulk carriers) → 
      SimpleBraidingOps.ad₀-simple carriers bulk-semiring 
      (SimpleBraidingOps.ad₂-simple carriers bulk-semiring t) ≡ 
      SimpleBraidingOps.ad₂-simple carriers bulk-semiring 
      (SimpleBraidingOps.ad₀-simple carriers bulk-semiring t)
    postulate postulate-comm-03 : ∀ (t : TrialityCarriers.Bulk carriers) → 
      SimpleBraidingOps.ad₀-simple carriers bulk-semiring 
      (SimpleBraidingOps.ad₃-simple carriers bulk-semiring t) ≡ 
      SimpleBraidingOps.ad₃-simple carriers bulk-semiring 
      (SimpleBraidingOps.ad₀-simple carriers bulk-semiring t)
    postulate postulate-comm-13 : ∀ (t : TrialityCarriers.Bulk carriers) → 
      SimpleBraidingOps.ad₁-simple carriers bulk-semiring 
      (SimpleBraidingOps.ad₃-simple carriers bulk-semiring t) ≡ 
      SimpleBraidingOps.ad₃-simple carriers bulk-semiring 
      (SimpleBraidingOps.ad₁-simple carriers bulk-semiring t)
    postulate postulate-braid-add : ∀ (t u : TrialityCarriers.Bulk carriers) → 
      SimpleBraidingOps.ad₀-simple carriers bulk-semiring (t ⊕B u) ≡ 
      SimpleBraidingOps.ad₀-simple carriers bulk-semiring t ⊕B 
      SimpleBraidingOps.ad₀-simple carriers bulk-semiring u
    postulate postulate-braid-mult : ∀ (t u : TrialityCarriers.Bulk carriers) → 
      SimpleBraidingOps.ad₀-simple carriers bulk-semiring (t ⊗B u) ≡ 
      SimpleBraidingOps.ad₀-simple carriers bulk-semiring t ⊗B 
      SimpleBraidingOps.ad₀-simple carriers bulk-semiring u
